\subsection*{Problem Statement}

Verify that $\surreal{n}{\omega - n}
= \surreal{1,2,...,(n - 1)}{\omega, \omega - 1, ..., \omega - (n - 1)}
= \frac{\omega}{2}$

\subsection*{Notes}
If $\surreal{n}{\omega - n} = \frac{\omega}{2}$ then $\surreal{n}{\omega - n} + \surreal{n}{\omega - n}=\omega$.  The definition of addition is:

\begin{equation*}
    x + y = \surreal{x^L + y, y^L + x}{x^R + y, y^R + x}
\end{equation*}

\begin{equation*}
    z = \{n|\omega - n\} + \{n|\omega - n\}
\end{equation*}

\begin{align*}
    x = & \surreal{n}{\omega - n} \\
    y = & \surreal{n}{\omega - n} \\
    X^L = & \{ 0, 1, 2 ... (n - 1) \} \\
    X^R = & \{ \omega, \omega - 1, \omega - 2, ... \omega - (n - 1) \}\\
    Y^L = & \{ 0, 1, 2 ... (n - 1) \} \\
    Y^R = & \{ \omega, \omega - 1, \omega - 2, ... \omega - (n - 1) \} \\
    X^L + y = & \{ (0 + \surreal{n}{\omega - n}), (1 + \surreal{n}{\omega - n}), ... (n - 1 + \surreal{n}{\omega - n}) \} \\
    Y^L + x = & \{ (0 + \surreal{n}{\omega - n}), (1 + \surreal{n}{\omega - n}), ... (n - 1 + \surreal{n}{\omega - n}) \} \\
    X^R + y = & \{ (\omega + \surreal{n}{\omega - n}), (\omega - 1 + \surreal{n}{\omega - n}), \\ & (\omega - 2 + \surreal{n}{\omega - n}), ... (\omega - (n - 1) + \surreal{n}{\omega - n}) \} \\
    Y^L + x = & \{ (\omega + \surreal{n}{\omega - n}), (\omega - 1 + \surreal{n}{\omega - n}), \\ & (\omega - 2 + \surreal{n}{\omega - n}), ... (\omega - (n - 1) + \surreal{n}{\omega - n}) \}
\end{align*}

The symmetry of the operation due to having the same term added to itself reduces the number of things to do here.  Furthermore, the two sets are already quite conveniently ordered, so the construction can be reduced to the greatest of the left and the least of the right:

\begin{align*}
    z = \surreal{n - 1 + \surreal{n}{\omega - n}}{\omega + \surreal{n}{\omega - n}}
\end{align*}

The question now is whether this expression is equal to $\omega$.

\surrealgeq{n - 1 + \surreal{n}{\omega - n}}{\omega + \surreal{n}{\omega - n}}{0, 1, 2, ...}{}

and

\surrealgeq{0, 1, 2, ...}{}{n - 1 + \surreal{n}{\omega - n}}{\omega + \surreal{n}{\omega - n}}