\documentclass{article}
\usepackage{amsmath}

\title{Concrete Math Chapter 2 Problem 27}
\author{Daniel Werner}

\begin{document}

\maketitle

\section*{Problem Statement}

Calculate $\Delta c^{\underline{x}}$ and use it to predict
the value of $\sum_1^n (-2)^{\underline{k}}/k$.

\section*{Solution}

\subsection*{Calculating $\Delta c^{\underline{x}}$}

\begin{align*}
    \Delta c^{\underline{x}} &= c^{\underline{x+1}} - c^{\underline{x}} \\
    &= c \cdot (c - 1) \cdot ... \cdot (c - X + 1) - 
    c \cdot (c - 1) \cdot ... \cdot (c - X)
\end{align*}

The product notation may make things easier to see,
 for $x \geq 0$ and ($c \geq x$ or $c \leq 0$):

 \begin{align*}
    c^{\underline{x+1}} - c^{\underline{x}}
    &= \prod_{0 \leq k \leq x} (c - k)
    - \prod_{0 \leq k \leq x - 1} (c - k) \\
    &= (c - x) \cdot \prod_{0 \leq k \leq x - 1} (c - k)
    - \prod_{0 \leq k \leq x - 1} (c - k) \\
    &= (c - x - 1) \cdot \prod_{0 \leq k \leq x - 1} (c - k)c \\
    &= (c - x - 1) \cdot ((c)(c-1)...(c-x+1)) \\
    &= \frac{(c)(c - 1)...(c - x + 1)(c - x)(c - x - 1)}{c - x} \\
    &= \frac{c^{\underline{x+2}}}{c - x}
 \end{align*}

 \subsection*{Some Testing}

 \begin{align*}
    5^{\underline{1+1}} - 5^{\underline{1}} &\stackrel{?}{=}
    \frac{5^{\underline{1+2}}}{5 - 1} \\
    5^{\underline{2}} - 5^{\underline{1}} &\stackrel{?}{=}
    \frac{5^{\underline{3}}}{4} \\
    5 * 4 - 5 &\stackrel{?}{=}
    \frac{5 * 4 * 3}{4} \\
    15 &= 15
 \end{align*}

 \begin{align*}
    11^{\underline{4+1}} - 11^{\underline{4}} &\stackrel{?}{=}
    \frac{11^{\underline{4 + 2}}}{11 - 4} \\
    11 * 10 * 9 * 8 * 7 - 11 * 10 * 9 * 8
    &\stackrel{?}{=} \frac{11 * 10 * 9 * 8 * 7 * 6}{ 7 } \\
    11 * 10 * 9 * 8 * 6
    &= 11 * 10 * 9 * 8 * 6
 \end{align*}

 \subsection*{Using $\Delta c^{\underline{x}}$ to solve the problem}

\begin{align*}
    \Delta c^{\underline{x}} = \frac{c^{\underline{x+2}}}{c - x}
    \rightarrow
    \Delta (-2)^{\underline{x}} = \frac{(-2)^{\underline{x+2}}}{-2 - x}
    \rightarrow
    \Delta (-2)^{\underline{x-2}} = \frac{2^{\underline{x}}}{-x}
\end{align*}

\begin{align*}
    \sum_1^n (-2)^{\underline{k}}/k
    = \left. \frac{(-2)^{\underline{x}}}{-x} \right|_1^{n+1}
    = \frac{(-2)^{\underline{n + 1}}}{-n - 1} 
    - \frac{(-2)^{\underline{1}}}{-1}
    = 2 - \frac{(-2)^{\underline{n+1}}}{n + 1}
\end{align*}

\end{document}